examples/unit-tests/unit1.fst
@@ -1,7 +1,7 @@
 (*--build-config
     options:--admit_fsi Set --verify_module Unit1;
     variables:LIB=../../lib;
-    other-files:$LIB/ext.fst $LIB/set.fsi $LIB/heap.fst $LIB/st.fst $LIB/list.fst $LIB/string.fst $LIB/int32.fst
+    other-files:$LIB/ext.fst $LIB/set.fsi $LIB/heap.fst $LIB/st.fst $LIB/list.fst $LIB/string.fst
 --*)
 module Unit1
 
